overhaul parser

C0deine/Parser/Basic.lean
@@ -1,124 +1,103 @@
 import Std
-import Parser
 
 import C0deine.Utils.Context
 import C0deine.Parser.Cst
+import C0deine.Parser.ParserT
 import C0deine.AuxDefs
-
-open Parser
 
 namespace C0deine.Parser
 
 
-abbrev C0Parser := SimpleParserT Substring Char (ExceptT (Parser.Error.Simple Substring Char) Context)
+abbrev C0Parser (s) := ParserT Context s
 
 namespace C0Parser
 
-/-- `notFollowedBy p` succeeds only if `p` fails -/
-@[inline] def _root_.Parser.notFollowedBy' {ε σ α β}
-  [Parser.Stream σ α] [Parser.Error ε σ α] {m} [Monad m] [MonadExceptOf ε m]
- (p : ParserT ε σ α m β) : ParserT ε σ α m Unit := do
-  try
-    let _ ← lookAhead p
-  catch _ =>
-    return
-  throwUnexpected
+open ParserT Cst
 
-def noBacktrackOr (p1 p2 : C0Parser α) := do
-  let oldPos ← getPosition
-  try p1
-  catch e =>
-    if (← getPosition) ≠ oldPos then
-      throw e
-    else
-      p2
+def intmin : Int := -2147483648
 
-notation p1 " </> " p2 => noBacktrackOr p1 p2
-
-open Cst
-
-instance : MonadLiftT Context C0Parser :=
-  show MonadLiftT _ (StateT _ _) from inferInstance
-instance : Inhabited (C0Parser α) := ⟨throwUnexpected⟩
-
-private def char (c : Char) : C0Parser Unit := do let _ ← Char.char c
-private def chars (s : String) : C0Parser Unit := do let _ ← Char.chars s
-
-def intmin : UInt32 := 0x80000000
-example : intmin.val = 1 <<< 31 := rfl
-
-def num : C0Parser UInt32 := do
-  dec </> hex </> (do let _ ← chars "-2147483648"; return intmin)
+def num : C0Parser s Int :=
+  first
+  [ dec
+  , hex
+  , (do char '0'; notFollowedBy (do let _ ← charMatching (·.isHexDigit)); return 0)
+  , (do wholeString "-2147483648"; return intmin)
+  ]
 where
-  dec : C0Parser UInt32 := do
-    let digs ← foldl String.push
-      (do let c ← tokenFilter (fun c => '1' ≤ c && c ≤ '9'); return c.toString)
-      (tokenFilter (fun c => '0' ≤ c && c ≤ '9'))
-    let nat := Nat.ofDigits? 10 digs |>.get!
-    if h : nat < intmin.val then
-      return ⟨nat, Nat.lt_trans h intmin.val.isLt⟩
-    else
-      throwUnexpected -- fun () => s!"int literal {digs} is too big"
-  hex : C0Parser UInt32 := do
-    char '0'
-    let _ ← (Char.char 'x' </> Char.char 'X')
-    let digs ← foldl String.push (pure "") (tokenFilter (fun c => '0' ≤ c && c ≤ '9' || 'a' ≤ c && c ≤ 'f' || 'A' ≤ c && c ≤ 'F'))
+  dec : C0Parser s Int := do
+    let digs ←
+      foldl
+        (do return (← charMatching (fun c => '1' ≤ c && c ≤ '9')).toString)
+        (fun acc => do
+          let c ← charMatching (fun c => '0' ≤ c && c ≤ '9')
+          return String.push acc c)
+    return Nat.ofDigits? 10 digs |>.get!
+  hex : C0Parser s Int := do
+    withBacktracking (do
+      char '0'
+      (char 'x' <|> char 'X')
+    )
+    let digs ←
+      foldl (return "") (fun s => do
+        let c ← charMatching (fun c => '0' ≤ c && c ≤ '9' || 'a' ≤ c && c ≤ 'f' || 'A' ≤ c && c ≤ 'F')
+        return s.push c)
     if digs.length = 0 then
       throwUnexpected -- fun () => "expected [0-9a-fA-F]"
     let nat := Nat.ofDigits? 16 digs |>.get!
-    if h : nat < intmin.val then
-      return ⟨nat, Nat.lt_trans h intmin.val.isLt⟩
-    else
-      throwUnexpected -- fun () => s!"int literal 0x{digs} is too big"
+    return nat
 
 
-def lineComment : C0Parser Unit := do
-  chars "//"
-  dropMany (tokenFilter (· ≠ '\n'))
+def lineComment : C0Parser s Unit := do
+  wholeString "//"
+  dropMany (do let _ ← charMatching (· ≠ '\n'))
 
-partial def blockComment : C0Parser Unit := do
-  chars "/*"
+partial def blockComment : C0Parser s Unit := do
+  wholeString "/*"
   dropMany (
-    (do let _ ← tokenFilter (¬ · ∈ ['/', '*']))
-    </> (do char '*'; notFollowedBy (do char '/'))
-    </> (do char '/'; notFollowedBy (do char '*'))
-    </> blockComment)
-  chars "*/"
+        (do let _ ← charMatching (¬ · ∈ ['/', '*']))
+    <|> (withBacktracking <| show C0Parser s _ from
+          do char '*'; notFollowedBy (char '/'))
+    <|> (withBacktracking <| show C0Parser s _ from
+          do char '/'; notFollowedBy (char '*'))
+    <|> blockComment)
+  wholeString "*/"
 
-def ws : C0Parser Unit :=
-  withErrorMessage "ws" <|
+def ws : C0Parser s Unit :=
+  withContext "ws" <|
   dropMany (
-    (do let _ ← tokenFilter (· ∈ [' ', '\n', '\t', '\r', '\u0011', '\u0012']))
-    </> lineComment
-    </> blockComment)
+    (withBacktracking <| show C0Parser _ _ from
+      do let a ← any; guard ((a : Char) ∈ [' ', '\n', '\t', '\r', '\u0011', '\u0012']))
+    <|> lineComment
+    <|> blockComment)
 
-@[inline] def keyword (s : String) : C0Parser Unit := withBacktracking do
+@[inline] def keyword (kw : String) : C0Parser s Unit := withBacktracking do
+  atomically (name := s!"\"{kw}\"") do
   /- keywords should not be followed by alphanums-/
-  chars s
-  notFollowedBy (tokenFilter (·.isAlphanum))
+  wholeString kw
+  notFollowedBy (do let _ ← charMatching (·.isAlphanum))
 
-def kw_struct       := keyword "struct"
-def kw_typedef      := keyword "typedef"
-def kw_if           := keyword "if"
-def kw_else         := keyword "else"
-def kw_while        := keyword "while"
-def kw_for          := keyword "for"
-def kw_continue     := keyword "continue"
-def kw_break        := keyword "break"
-def kw_return       := keyword "return"
-def kw_assert       := keyword "assert"
-def kw_true         := keyword "true"
-def kw_false        := keyword "false"
-def kw_NULL         := keyword "NULL"
-def kw_alloc        := keyword "alloc"
-def kw_alloc_array  := keyword "alloc_array"
-def kw_int          := keyword "int"
-def kw_bool         := keyword "bool"
-def kw_void         := keyword "void"
-def kw_char         := keyword "char"
-def kw_string       := keyword "string"
+def kw_struct       : C0Parser s Unit := keyword "struct"
+def kw_typedef      : C0Parser s Unit := keyword "typedef"
+def kw_if           : C0Parser s Unit := keyword "if"
+def kw_else         : C0Parser s Unit := keyword "else"
+def kw_while        : C0Parser s Unit := keyword "while"
+def kw_for          : C0Parser s Unit := keyword "for"
+def kw_continue     : C0Parser s Unit := keyword "continue"
+def kw_break        : C0Parser s Unit := keyword "break"
+def kw_return       : C0Parser s Unit := keyword "return"
+def kw_assert       : C0Parser s Unit := keyword "assert"
+def kw_true         : C0Parser s Unit := keyword "true"
+def kw_false        : C0Parser s Unit := keyword "false"
+def kw_NULL         : C0Parser s Unit := keyword "NULL"
+def kw_alloc        : C0Parser s Unit := keyword "alloc"
+def kw_alloc_array  : C0Parser s Unit := keyword "alloc_array"
+def kw_int          : C0Parser s Unit := keyword "int"
+def kw_bool         : C0Parser s Unit := keyword "bool"
+def kw_void         : C0Parser s Unit := keyword "void"
+def kw_char         : C0Parser s Unit := keyword "char"
+def kw_string       : C0Parser s Unit := keyword "string"
 
-def anyKeyword : C0Parser Unit :=
+def anyKeyword : C0Parser s Unit :=
   first [
     kw_struct
   , kw_typedef
@@ -144,22 +123,24 @@ def anyKeyword : C0Parser Unit :=
 
 variable (tydefs : Std.RBSet Symbol Ord.compare)
 
-def rawIdent : C0Parser Ident := do
-  notFollowedBy' anyToken --anyKeyword
-  let c ← tokenFilter (fun c => c.isAlpha || c = '_')
-  let str ← foldl String.push (return c.toString) (tokenFilter (fun c => c.isAlphanum || c = '_'))
+def rawIdent : C0Parser s Ident := do
+  notFollowedBy anyKeyword
+  let c ← charMatching (fun c => c.isAlpha || c = '_')
+  let str ← foldl (return c.toString) (fun s => do
+    let c ← charMatching (fun c => c.isAlphanum || c = '_')
+    return s.push c)
   return ← liftM <| Symbol.symbol str
 
-def typeIdent : C0Parser Ident :=
-  withErrorMessage "<type-ident>" do
+def typeIdent : C0Parser s Ident :=
+  withContext "<type-ident>" do
   let id ← rawIdent
   if tydefs.contains id then
     return id
   else
     throwUnexpected
 
-def ident : C0Parser Ident :=
-  withErrorMessage "<ident>" do
+def ident : C0Parser s Ident :=
+  withContext "<ident>" do
   let id ← rawIdent
   if tydefs.contains id then
     throwUnexpected
@@ -168,278 +149,298 @@ def ident : C0Parser Ident :=
 
 
 mutual
-def simpleTyp : C0Parser Typ :=
+def simpleTyp : C0Parser s Typ :=
       (do kw_int ; return Typ.int)
-  </> (do kw_bool; return Typ.bool)
-  </> (do kw_void; return Typ.void)
-  </> (do let name ← ident tydefs; return Typ.tydef name)
-  </> (do kw_struct; ws; let name ← ident tydefs; return Typ.struct name)
+  <|> (do kw_bool; return Typ.bool)
+  <|> (do kw_void; return Typ.void)
+  <|> (do let name ← ident tydefs; return Typ.tydef name)
+  <|> (do kw_struct; ws; let name ← rawIdent; return Typ.struct name)
 
-def typ : C0Parser Typ :=
-  withErrorMessage "<type>" do
+def typ : C0Parser s Typ :=
+  withContext "<type>" do
   -- parse a simple type
   let t ← simpleTyp
   -- parse as many * and [] as we can
-  foldl (fun t (f : Typ → Typ) => f t)
-    (return t)
-    (do
-      ws
-      (do char '*'; return Typ.ptr)
-      </> (do char '['; ws; char ']'; return Typ.arr) )
+  foldl (return t)
+    (fun t =>
+      (do withBacktracking (do ws; char '*'); return Typ.ptr t)
+      <|> (do withBacktracking (do ws; char '['); ws; char ']'; return Typ.arr t) )
 end
 
-def unop.int : C0Parser UnOp.Int :=
+def unop.int : C0Parser s UnOp.Int :=
   (do char '-'; notFollowedBy (char '-'); notFollowedBy (char '>'); return .neg)
-  </> (do char '~'; return .not)
+  <|> (do char '~'; return .not)
 
-def unop.bool : C0Parser UnOp.Bool :=
+def unop.bool : C0Parser s UnOp.Bool :=
   (do char '!'; return .not)
 
-def unop : C0Parser UnOp :=
+def unop : C0Parser s UnOp :=
     (do let op ← unop.int; return .int op)
-</> (do let op ← unop.bool; return .bool op)
+<|> (do let op ← unop.bool; return .bool op)
 
-def binop.int.prec_11 : C0Parser BinOp.Int :=
+def binop.int.prec_11 : C0Parser s BinOp.Int :=
      (do char '*'; return .times)
-</> (do char '/'; return .div)
-</> (do char '%'; return .mod)
+<|> (do char '/'; return .div)
+<|> (do char '%'; return .mod)
 
-def binop.int.prec_10 : C0Parser BinOp.Int :=
+def binop.int.prec_10 : C0Parser s BinOp.Int :=
     (do char '+'; return .plus)
-</> (do char '-'; notFollowedBy (char '-'); return .minus)
+<|> (do char '-'; notFollowedBy (char '-'); return .minus)
 
-def binop.int.prec_9 : C0Parser BinOp.Int :=
-    (do chars "<<"; return .lsh)
-</> (do chars ">>"; return .rsh)
+def binop.int.prec_9 : C0Parser s BinOp.Int :=
+    (do wholeString "<<"; return .lsh)
+<|> (do wholeString ">>"; return .rsh)
 
-def binop.cmp.prec_8 : C0Parser BinOp.Cmp :=
+def binop.cmp.prec_8 : C0Parser s BinOp.Cmp :=
     (do char '<'; return .lt)
-</> (do chars "<="; return .le)
-</> (do char '>'; return .gt)
-</> (do chars ">="; return .ge)
+<|> (do wholeString "<="; return .le)
+<|> (do char '>'; return .gt)
+<|> (do wholeString ">="; return .ge)
 
-def binop.cmp.prec_7 : C0Parser BinOp.Cmp :=
-    (do chars "=="; return .eq)
-</> (do chars "!="; return .ne)
+def binop.cmp.prec_7 : C0Parser s BinOp.Cmp :=
+    (do wholeString "=="; return .eq)
+<|> (do wholeString "!="; return .ne)
 
-def binop.int.prec_6 : C0Parser BinOp.Int :=
+def binop.int.prec_6 : C0Parser s BinOp.Int :=
   (do char '&'; return .and)
 
-def binop.int.prec_5 : C0Parser BinOp.Int :=
+def binop.int.prec_5 : C0Parser s BinOp.Int :=
   (do char '^'; return .xor)
 
-def binop.int.prec_4 : C0Parser BinOp.Int :=
+def binop.int.prec_4 : C0Parser s BinOp.Int :=
   (do char '|'; return .or)
 
-def binop.bool.prec_3 : C0Parser BinOp.Bool :=
-  (do chars "&&"; return .and)
+def binop.bool.prec_3 : C0Parser s BinOp.Bool :=
+  (do wholeString "&&"; return .and)
 
-def binop.bool.prec_2 : C0Parser BinOp.Bool :=
-  (do chars "||"; return .or)
+def binop.bool.prec_2 : C0Parser s BinOp.Bool :=
+  (do wholeString "||"; return .or)
 
-def binop.int : C0Parser BinOp.Int :=
-  binop.int.prec_11 </> binop.int.prec_10 </> binop.int.prec_9
-  </> binop.int.prec_6 </> binop.int.prec_5 </> binop.int.prec_4
+def binop.int : C0Parser s BinOp.Int :=
+  binop.int.prec_11 <|> binop.int.prec_10 <|> binop.int.prec_9
+  <|> binop.int.prec_6 <|> binop.int.prec_5 <|> binop.int.prec_4
 
-def asnop : C0Parser AsnOp :=
+def asnop : C0Parser s AsnOp :=
     (do char '='; return .eq)
-</> (do let op ← binop.int; char '='; return .aseq op)
+<|> (do let op ← binop.int; char '='; return .aseq op)
 
-def postop : C0Parser PostOp :=
-    (do chars "++"; return .incr)
-</> (do chars "--"; return .decr)
+def postop : C0Parser s PostOp :=
+    (do wholeString "++"; return .incr)
+<|> (do wholeString "--"; return .decr)
 
 mutual
-partial def lvalue : C0Parser LValue :=
-  foldl (fun x (f : LValue → LValue) => f x)
+partial def lvalue : C0Parser s LValue :=
+  foldl
     (do let name ← ident tydefs; return .var name)
-    (do
+    (fun lv => do
       ws
       (do
         char '.'; ws
         let field ← ident tydefs
-        return (.dot · field))
-      </> (do
-        chars "->"; ws
+        return (.dot lv field))
+      <|> (do
+        wholeString "->"; ws
         let field ← ident tydefs
-        return (.arrow · field))
-      </> (do
+        return (.arrow lv field))
+      <|> (do
         char '*'; ws
-        return (.deref ·))
-      </> (do
+        return (.deref lv))
+      <|> (do
         char '['; ws; let index ← expr; char ']'
-        return (.index · index))
+        return (.index lv index))
     )
 
-partial def expr.prec_13.left : C0Parser Expr :=
+partial def expr.prec_13.left : C0Parser s Expr :=
     (do let v ← num; return .num v)
-</> (do kw_true; return .«true»)
-</> (do kw_false; return .«false»)
-</> (do kw_NULL; return .null)
-</> (do kw_alloc; ws; char '('; ws
+<|> (do kw_true; return .«true»)
+<|> (do kw_false; return .«false»)
+<|> (do kw_NULL; return .null)
+<|> (do kw_alloc; ws; char '('; ws
         let ty ← typ tydefs
         ws; char ')'
         return .alloc ty)
-</> (do kw_alloc_array; ws; char '('; ws
+<|> (do kw_alloc_array; ws; char '('; ws
         let ty ← typ tydefs
         ws; char ','; ws
         let e ← expr
         ws; char ')'
         return .alloc_array ty e)
-</> (do let name ← ident tydefs
+<|> (do let name ← ident tydefs
         (do ws; char '('; ws
-            let args ← foldl (Array.push)
+            let args ← foldl
               (do let e ← expr; return #[e])
-              (do ws; char ','; ws; expr)
+              (fun acc => do ws; char ','; ws; return acc.push (← expr))
             char ')'
             return .app name args.toList)
-        </>
+        <|>
         (return .var name))
-</> (do char '('; let e ← expr; char ')'; return e)
+<|> (do char '('; let e ← expr; char ')'; return e)
 
-partial def expr.prec_13 : C0Parser Expr :=
-  foldl (fun x (f : Expr → Expr) => f x) expr.prec_13.left
-    (   (do ws; char '.'  ; ws; let f ← ident tydefs; return (.dot · f))
-    </> (do ws; chars "->"; ws; let f ← ident tydefs; return (.arrow · f))
-    </> (do ws; char '['  ; ws; let e ← expr; return (.index · e)))
+partial def expr.prec_13 : C0Parser s Expr :=
+  foldl expr.prec_13.left (fun lhs =>
+        (do ws; char '.'  ; ws; let f ← ident tydefs
+            return (.dot lhs f))
+    <|> (do ws; wholeString "->"; ws; let f ← ident tydefs
+            return (.arrow lhs f))
+    <|> (do ws; char '['  ; ws; let e ← expr
+            return (.index lhs e)))
 
-partial def expr.prec_12 : C0Parser Expr :=
+partial def expr.prec_12 : C0Parser s Expr :=
     (do let op ← unop; ws; return .unop op (← expr.prec_12))
-</> (do char '*'; ws; return .deref (← expr.prec_12))
-</> expr.prec_13
+<|> (do char '*'; ws; return .deref (← expr.prec_12))
+<|> expr.prec_13
 
-partial def expr.prec_11 : C0Parser Expr :=
-  foldl (fun x (f : Expr → Expr) => f x) expr.prec_12
-    (do ws; let op ← binop.int.prec_11; ws; let rhs ← expr.prec_12; return (.binop (.int op) · rhs))
+partial def expr.prec_11 : C0Parser s Expr :=
+  foldl expr.prec_12 (fun lhs => do
+    ws; let op ← binop.int.prec_11; ws; let rhs ← expr.prec_12
+    return (.binop (.int op) lhs rhs))
 
-partial def expr.prec_10 : C0Parser Expr :=
-  foldl (fun x (f : Expr → Expr) => f x) expr.prec_11
-    (do ws; let op ← binop.int.prec_10; ws; let rhs ← expr.prec_11; return (.binop (.int op) · rhs))
+partial def expr.prec_10 : C0Parser s Expr :=
+  foldl expr.prec_11 (fun lhs => do
+    ws; let op ← binop.int.prec_10; ws; let rhs ← expr.prec_11
+    return (.binop (.int op) lhs rhs))
 
-partial def expr.prec_9 : C0Parser Expr :=
-  foldl (fun x (f : Expr → Expr) => f x) expr.prec_10
-    (do ws; let op ← binop.int.prec_9; ws; let rhs ← expr.prec_10; return (.binop (.int op) · rhs))
+partial def expr.prec_9 : C0Parser s Expr :=
+  foldl expr.prec_10 (fun lhs => do
+    ws; let op ← binop.int.prec_9; ws; let rhs ← expr.prec_10
+    return (.binop (.int op) lhs rhs))
 
-partial def expr.prec_8 : C0Parser Expr :=
-  foldl (fun x (f : Expr → Expr) => f x) expr.prec_9
-    (do ws; let op ← binop.cmp.prec_8; ws; let rhs ← expr.prec_9; return (.binop (.cmp op) · rhs))
+partial def expr.prec_8 : C0Parser s Expr :=
+  foldl expr.prec_9 (fun lhs => do
+    ws; let op ← binop.cmp.prec_8; ws; let rhs ← expr.prec_9
+    return (.binop (.cmp op) lhs rhs))
 
-partial def expr.prec_7 : C0Parser Expr :=
-  foldl (fun x (f : Expr → Expr) => f x) expr.prec_8
-    (do ws; let op ← binop.cmp.prec_7; ws; let rhs ← expr.prec_8; return (.binop (.cmp op) · rhs))
+partial def expr.prec_7 : C0Parser s Expr :=
+  foldl expr.prec_8 (fun lhs => do
+    ws; let op ← binop.cmp.prec_7; ws; let rhs ← expr.prec_8
+    return (.binop (.cmp op) lhs rhs))
 
-partial def expr.prec_6 : C0Parser Expr :=
-  foldl (fun x (f : Expr → Expr) => f x) expr.prec_7
-    (do ws; let op ← binop.int.prec_6; ws; let rhs ← expr.prec_7; return (.binop (.int op) · rhs))
+partial def expr.prec_6 : C0Parser s Expr :=
+  foldl expr.prec_7 (fun lhs => do
+    ws; let op ← binop.int.prec_6; ws; let rhs ← expr.prec_7
+    return (.binop (.int op) lhs rhs))
 
-partial def expr.prec_5 : C0Parser Expr :=
-  foldl (fun x (f : Expr → Expr) => f x) expr.prec_6
-    (do ws; let op ← binop.int.prec_5; ws; let rhs ← expr.prec_6; return (.binop (.int op) · rhs))
+partial def expr.prec_5 : C0Parser s Expr :=
+  foldl expr.prec_6 (fun lhs => do
+    ws; let op ← binop.int.prec_5; ws; let rhs ← expr.prec_6
+    return (.binop (.int op) lhs rhs))
 
-partial def expr.prec_4 : C0Parser Expr :=
-  foldl (fun x (f : Expr → Expr) => f x) expr.prec_5
-    (do ws; let op ← binop.int.prec_4; ws; let rhs ← expr.prec_5; return (.binop (.int op) · rhs))
+partial def expr.prec_4 : C0Parser s Expr :=
+  foldl expr.prec_5 (fun lhs => do
+    ws; let op ← binop.int.prec_4; ws; let rhs ← expr.prec_5
+    return (.binop (.int op) lhs rhs))
 
-partial def expr.prec_3 : C0Parser Expr :=
-  foldl (fun x (f : Expr → Expr) => f x) expr.prec_4
-    (do ws; let op ← binop.bool.prec_3; ws; let rhs ← expr.prec_4; return (.binop (.bool op) · rhs))
+partial def expr.prec_3 : C0Parser s Expr :=
+  foldl expr.prec_4 (fun lhs => do
+    ws; let op ← binop.bool.prec_3; ws; let rhs ← expr.prec_4
+    return (.binop (.bool op) lhs rhs))
 
-partial def expr.prec_2 : C0Parser Expr :=
-  foldl (fun x (f : Expr → Expr) => f x) expr.prec_3
-    (do ws; let op ← binop.bool.prec_2; ws; let rhs ← expr.prec_3; return (.binop (.bool op) · rhs))
+partial def expr.prec_2 : C0Parser s Expr :=
+  foldl expr.prec_3 (fun lhs => do
+    ws; let op ← binop.bool.prec_2; ws; let rhs ← expr.prec_3
+    return (.binop (.bool op) lhs rhs))
 
-partial def expr.prec_1 : C0Parser Expr := do
+partial def expr.prec_1 : C0Parser s Expr := do
   let lhs ← expr.prec_2
-  (do ws; char '?'; ws; let tt ← expr.prec_1; ws; char ':'; ws; let ff ← expr.prec_1;
+  (do withBacktracking (ws *> char '?'); ws
+      let tt ← expr.prec_1; ws
+      char ':'; ws; let ff ← expr.prec_1;
       return .ternop lhs tt ff)
-  </> (do return lhs)
+  <|> (do return lhs)
 
-partial def expr : C0Parser Expr := expr.prec_1
+partial def expr : C0Parser s Expr := expr.prec_1
 end
 
 mutual
-partial def control : C0Parser Control :=
+partial def control : C0Parser s Control :=
     (do kw_if; ws; char '('; ws; let cond ← expr tydefs; ws; char ')'; ws
         let tt ← stmt
-        let ff ← option? (do ws; kw_else; stmt)
+        let ff ← option (do withBacktracking (do ws; kw_else); stmt)
         return Control.ite cond tt (ff.getD (.block [])))
-</> (do kw_while; ws; char '('; ws; let cond ← expr tydefs; ws; char ')'; ws
+<|> (do kw_while; ws; char '('; ws; let cond ← expr tydefs; ws; char ')'; ws
         let body ← stmt
         return Control.«while» cond body)
-</> (do kw_for; ws; char '('; ws;
-        let init ← simp; ws; char ';'; ws; let cond ← expr tydefs; ws; char ';'; ws; let step ← option? simp; ws; char ')'; ws
+<|> (do kw_for; ws; char '('; ws
+        let init ← simp; ws; char ';'; ws
+        let cond ← expr tydefs; ws; char ';'; ws
+        let step ← option simp; ws
+        char ')'; ws
         let body ← stmt
         return Control.«for» init cond step body)
-</> (do kw_return; ws; let e ← option? (expr tydefs); ws; char ';'
+<|> (do kw_return; ws; let e ← option (expr tydefs); ws; char ';'
         return Control.«return» e)
-</> (do kw_assert; ws; let e ← expr tydefs; ws; char ';'
+<|> (do kw_assert; ws; let e ← expr tydefs; ws; char ';'
         return Control.assert e)
 
-partial def simp : C0Parser Simp :=
+partial def simp : C0Parser s Simp :=
     (do let type ← typ tydefs; ws
         let name ← ident tydefs; ws;
-        let init ← option? (do char '='; ws; expr tydefs)
+        let init ← option (do char '='; ws; expr tydefs)
         return .decl type name init)
-</> (do let lv ← lvalue tydefs; ws
+<|> (do let lv ← lvalue tydefs; ws
         let op ← asnop; ws
         let v ← expr tydefs
         return .assn lv op v)
-</> (do let lv ← lvalue tydefs; ws
+<|> (do let lv ← lvalue tydefs; ws
         let op ← postop
         return .post lv op)
-</> (do let e ← expr tydefs; return .exp e)
+<|> (do let e ← expr tydefs; return .exp e)
 
-partial def block : C0Parser Stmt :=
-    (do char '{'; ws; char '}'
-        return .block [])
-</> (do char '{'; ws
-        let body ← sepBy ws stmt
-        ws; char '}'
-        return .block body.toList)
+partial def block : C0Parser s Stmt :=
+  (do char '{'; ws
+      let body ← sepBy ws stmt
+      ws; char '}'
+      return .block body.toList)
 
-partial def stmt : C0Parser Stmt :=
+partial def stmt : C0Parser s Stmt :=
     (do let s ← simp; ws; char ';'; return .simp s)
-</> (do return .ctrl (←control))
-</> block
+<|> (do return .ctrl (←control))
+<|> block
 end
 
-def field : C0Parser Field := do
+def field : C0Parser s Field :=
+  withContext "<struct-field>" do
   let type ← typ tydefs
   ws
   let name ← ident tydefs
   char ';'
   return ⟨type, name⟩
 
-def sdef : C0Parser SDef :=
-  withErrorMessage "<struct-def>" do
-  kw_struct; ws
-  let name ← ident tydefs; ws
-  char '{'; ws
+def sdef : C0Parser s SDef :=
+  withContext "<struct-def>" do
+  let name ← withBacktracking do
+    kw_struct; ws
+    let name ← ident tydefs; ws
+    char '{'
+    pure name
+  ws
   let fields ← sepBy ws (field tydefs)
   ws; char '}'; char ';'
   return ⟨name, fields.toList⟩
 
-def sdecl : C0Parser SDecl :=
-  withErrorMessage "<struct-decl>" do
+def sdecl : C0Parser s SDecl :=
+  withContext "<struct-decl>" <|
+  withBacktracking do
   kw_struct; ws
   let name ← ident tydefs; ws
   char ';'
   return ⟨name⟩
 
-def tydef : C0Parser TyDef :=
-  withErrorMessage "<type-def>" do
+def tydef : C0Parser s TyDef :=
+  withContext "<type-def>" do
   kw_typedef; ws
   let type ← typ tydefs; ws
   let name ← ident tydefs; ws
   char ';'
   return ⟨type, name⟩
 
-def param : C0Parser Param := do
+def param : C0Parser s Param := do
   let type ← typ tydefs; ws
   let name ← ident tydefs
   return ⟨type, name⟩
 
-private def signature : C0Parser FDecl := do
+private def signature : C0Parser s FDecl :=
+  withContext "<func-sig>" do
   let type ← typ tydefs; ws
   let name ← ident tydefs; ws
   char '('; ws
@@ -447,34 +448,35 @@ private def signature : C0Parser FDecl := do
   ws; char ')'
   return ⟨type, name, params.toList⟩
 
-def fdecl : C0Parser FDecl :=
-  withErrorMessage "<func-decl>" do
-  let sig ← signature tydefs
+def fdecl (sig : FDecl) : C0Parser s FDecl :=
+  withContext "<func-decl>" <|
+  withBacktracking do
   ws; char ';'
   return sig
 
-def fdef : C0Parser FDef :=
-  withErrorMessage "<func-def>" do
-  let sig ← signature tydefs
+def fdef (sig : FDecl) : C0Parser s FDef :=
+  withContext "<func-def>" do
   ws
   let body ← block tydefs
   return {sig with body}
 
-def gdecl : C0Parser GDecl :=
-    (do return .fdecl (← fdecl tydefs)) 
-</> (do return .tydef (← tydef tydefs))
-</> (do return .sdecl (← sdecl tydefs))
-</> (do return .sdef  (← sdef  tydefs)) 
-</> (do return .fdef  (← fdef  tydefs))
+def gdecl : C0Parser s GDecl :=
+  first
+  [do return .tydef (← tydef tydefs)
+  ,do return .sdecl (← sdecl tydefs)
+  ,do return .sdef  (← sdef  tydefs)
+  ,do let sig ← signature tydefs
+      (return .fdecl (← fdecl sig)) 
+      <|> (return .fdef (← fdef tydefs sig))
+  ]
 
-partial def prog : C0Parser Prog :=
-  withErrorMessage "<prog>" do
+partial def prog : C0Parser s Prog := do
   ws
   let gdecls ← aux (Std.RBSet.empty) #[]
   return gdecls.toList
 where aux tydefs acc :=
-  (do Parser.endOfInput; return acc)
-  </> (do
+  (do eof; return acc)
+  <|> (do
     let g ← gdecl tydefs
     ws
     let tydefs := match g with | .tydef ⟨_, i⟩ => tydefs.insert i | _ => tydefs
