C0deine/AuxDefs.lean
@@ -37,3 +37,92 @@ def Nat.ofDigits? (base : Nat) (s : String) : Option Nat :=
       else
         none)
     (some 0)
+
+@[simp] theorem UInt32.toNat_ofUInt8 : UInt32.toNat (UInt8.toUInt32 x) = x.val := by
+  cases x; case mk val =>
+  cases val; case mk val isLt =>
+  have : val < 4294967295 + 1 := Nat.le_trans isLt (by decide)
+  simp [UInt8.size] at isLt
+  simp only [toNat]
+  apply Nat.mod_eq_of_lt this
+
+instance : Coe UInt8 Char where
+  coe b := ⟨UInt8.toUInt32 b, by
+    rcases b with ⟨⟨x,h⟩⟩
+    apply Or.inl
+    simp
+    apply Nat.lt_trans h (by decide)
+  ⟩
+
+def Char.toUInt8 (c : Char) (h : c.val.val < UInt8.size := by decide) : UInt8 :=
+  ⟨c.val.val, h⟩
+
+instance (h : c.val.val < UInt8.size := by decide) : CoeDep Char c UInt8 := ⟨c.toUInt8 h⟩
+
+structure ThunkCache (a : Unit → α) where
+  val : Thunk α
+  h_val : val.get = a ()
+
+def ThunkCache.new : ThunkCache a := ⟨Thunk.mk a, by simp [Thunk.get]⟩
+instance : Inhabited (ThunkCache a) := ⟨.new⟩
+
+def List.pmap (L : List α) (f : (a : α) → a ∈ L → β) : List β :=
+  match L with
+  | [] => []
+  | x::xs => (f x (List.Mem.head _)) :: xs.pmap (fun a h => f a (List.Mem.tail _ h))
+
+@[simp] theorem String.length_pushn (s : String) (c n)
+  : (s.pushn c n).length = s.length + n := by
+  induction n
+  . simp [pushn, Nat.repeat]
+  . simp [pushn, Nat.repeat, push, length]
+    rw [Nat.add_succ, Nat.add_succ]
+    congr
+
+@[simp] theorem String.length_append (s1 s2 : String)
+  : (s1 ++ s2).length = s1.length + s2.length := by
+  simp [HAppend.hAppend, Append.append, append, length]
+
+@[simp] theorem String.take_mk (L : List Char) (n)
+  : (String.mk L).take n = String.mk (L.take n)
+  := sorry
+
+@[simp] theorem String.drop_mk (L : List Char) (n)
+  : (String.mk L).drop n = String.mk (L.drop n)
+  := sorry
+
+@[simp] theorem String.length_take (s : String) (n)
+  : (s.take n).length = min s.length n
+  := by cases s; simp [length, Nat.min_comm]
+
+@[simp] theorem String.length_drop (s : String) (n)
+  : (s.drop n).length = s.length - n
+  := by cases s; simp [length, Nat.min_comm]
+
+theorem List.mem_zipWith (h : x ∈ List.zipWith f L1 L2)
+  : ∃ y z, x = f y z ∧ y ∈ L1 ∧ z ∈ L2
+  := by induction L1 generalizing x L2
+        . simp at h
+        . next ih =>
+          cases L2 <;> simp at *
+          cases h
+          . subst_vars
+            exact ⟨_, _, rfl, .inl rfl, .inl rfl⟩
+          . have := ih (by assumption)
+            rcases this with ⟨y,z,rfl,hy,hz⟩
+            refine ⟨y,z, rfl, .inr hy, .inr hz⟩
+
+theorem List.mem_take (h : x ∈ List.take n L)
+  : x ∈ L
+  := by induction n generalizing L <;> cases L <;> simp at *
+        next ih _ _ =>
+        cases h
+        . apply Or.inl; assumption
+        . apply Or.inr; apply ih; assumption
+
+@[simp]
+theorem List.length_join_replicate : (replicate n L).join.length = n * L.length := by
+  induction n
+  . simp
+  . simp [Nat.succ_mul, Nat.add_comm]
+    congr
