C0deine/Utils/CliFormat.lean
@@ -1,0 +1,253 @@
+import C0deine.AuxDefs
+
+namespace C0deine.Utils.CliFormat
+
+structure Rect where
+  (width height : Nat)
+  lines : List String
+  h_height : lines.length = height
+  h_width : ∀ l, l ∈ lines → l.length = width
+
+def Rect.ofLines (lines : List String) : Rect :=
+  let width := lines.foldr (max ·.length) 0
+  have : ∀ l, l ∈ lines → l.length ≤ width := by
+    intro l hl
+    induction lines
+    . simp at hl
+    . simp at hl ⊢
+      cases hl
+      . simp [*, Nat.le_max_left]
+      . apply Nat.le_trans _ (Nat.le_max_right ..)
+        simp [*] at *
+  { width, height := lines.length
+  , lines := lines.map (fun l => l.pushn ' ' (width - l.length))
+  , h_height := by simp, h_width := by
+      intro l h
+      rw [List.mem_map] at h
+      rcases h with ⟨l',hl',rfl⟩
+      simp; rw [Nat.add_comm]
+      apply Nat.sub_add_cancel
+      apply this _ hl' 
+  }
+
+def Rect.ofString (s : String) : Rect :=
+  have lines := s.splitOn "\n"
+  Rect.ofLines lines
+
+instance : Coe Char Rect where
+  coe c := .ofString c.toString
+
+instance : Coe String Rect where
+  coe s := .ofString s
+
+instance : Coe (List String) Rect where
+  coe l := .ofLines l
+
+instance : Coe Rect String where
+  coe r := String.intercalate "\n" r.lines
+
+inductive HAlign | left | center | right
+inductive VAlign | top | center | bottom
+
+def Rect.padHeight (r : Rect) (height : Nat) (h_height : r.height ≤ height)
+                  (align : VAlign) : Rect :=
+  { height, width := r.width
+  , lines :=
+    match align with
+    | .top    => r.lines ++ List.replicate (height - r.height) ("".pushn ' ' r.width)
+    | .bottom => List.replicate (height - r.height) ("".pushn ' ' r.width) ++ r.lines
+    | .center => let top := (height - r.height)/2
+                 List.replicate top ("".pushn ' ' r.width) ++ r.lines ++
+                 List.replicate (height - r.height - top) ("".pushn ' ' r.width)
+  , h_height := by
+      split <;> simp [r.h_height]
+      . apply Nat.add_sub_cancel' h_height
+      . apply Nat.sub_add_cancel h_height
+      . rw [← Nat.add_assoc, Nat.sub_sub, Nat.add_comm r.height]
+        apply Nat.add_sub_cancel'
+        apply Nat.add_le_of_le_sub h_height
+        apply Nat.div_le_self
+  , h_width := by
+      intro l h
+      cases align <;> (
+        simp at h
+        cases h <;> (try rename _ ∨ _ => h; cases h) <;>
+          first
+          | (apply r.h_width; assumption)
+          | (have := List.mem_replicate.mp (by assumption) |>.2
+             cases this; simp; simp [String.length])
+        )
+  }
+
+def Rect.padWidth (r : Rect) (width : Nat) (h_width : r.width ≤ width)
+                  (align : HAlign) : Rect :=
+  { width, height := r.height
+  , lines := r.lines.map (fun l => 
+    match align with
+    | .left   => l.pushn ' ' (width - l.length)
+    | .right  => "".pushn ' ' (width - l.length) ++ l
+    | .center => let left := (width - l.length)/2
+                 "".pushn ' ' left ++ l |>.pushn ' ' (width-l.length-left)
+    )
+  , h_height := by simp [r.h_height], h_width := by
+      intros; have := List.mem_map.mp (by assumption)
+      match this with
+      | ⟨line,hmem,_⟩ =>
+      have := r.h_width _ hmem
+      cases align <;> simp [*]
+      . apply Nat.add_sub_cancel' h_width
+      . simp [String.length]; rw [Nat.sub_sub, Nat.add_comm r.width]
+        apply Nat.add_sub_cancel'
+        apply Nat.add_le_of_le_sub h_width
+        apply Nat.div_le_self
+      . simp [String.length]; apply Nat.sub_add_cancel h_width
+  }
+
+def Rect.joinVert (top bottom : Rect) (h : top.width = bottom.width) : Rect :=
+  { width := top.width, height := top.height + bottom.height
+  , lines := top.lines ++ bottom.lines
+  , h_height := by simp [top.h_height, bottom.h_height]
+  , h_width := by simp (config := {contextual := true}) [or_imp, h, top.h_width, bottom.h_width]}
+
+def Rect.joinHorz (left right : Rect) (h : left.height = right.height) : Rect :=
+  { height := left.height, width := left.width + right.width
+  , lines := List.zipWith (· ++ ·) left.lines right.lines
+  , h_height := by simp [left.h_height, right.h_height, h]; apply Nat.min_eq_left (Nat.le_refl _)
+  , h_width := by intro l hl; have := List.mem_zipWith hl
+                  rcases this with ⟨y,z, rfl, hy, hz⟩
+                  simp [left.h_width _ hy, right.h_width _ hz]}
+
+def empty : Rect := { width := 0, height := 0, lines := [], h_width := by simp, h_height := by simp }
+
+def fill (c : Char) (width height : Nat) : Rect :=
+  { width, height, lines := List.replicate height ("".pushn c width)
+  , h_width := by intro l hl; have := List.mem_replicate.mp hl; simp [this]; simp [String.length]
+  , h_height := by simp }
+
+def space (width height : Nat) : Rect :=
+  fill ' ' width height
+
+@[simp] theorem space.width_eq : (space w h).width = w := by
+  simp [space, fill]
+
+@[simp] theorem space.height_eq : (space w h).height = h := by
+  simp [space, fill]
+
+def Rect.trimHeight (height : Nat) (r : Rect) : Rect :=
+  { width := r.width, height := min r.height height
+  , lines := r.lines.take height
+  , h_width := by intro l hl; have := List.mem_take hl; apply r.h_width _ this
+  , h_height := by simp [r.h_height, Nat.min_comm] }
+
+def Rect.trimWidth (width : Nat) (r : Rect) : Rect :=
+  { width := min r.width width, height := r.height
+  , lines := r.lines.map (·.take width)
+  , h_width := by intro l hl; have := List.mem_map.mp hl
+                  rcases this with ⟨a, ha, rfl⟩
+                  simp [r.h_width _ ha]
+  , h_height := by simp [r.h_height, Nat.min_comm] }
+
+def Rect.dropLeft (n : Nat)  (r : Rect): Rect :=
+  { width := r.width - n, height := r.height
+  , lines := r.lines.map (·.drop n)
+  , h_width := by intro l hl; have := List.mem_map.mp hl
+                  rcases this with ⟨a,ha,rfl⟩
+                  simp [r.h_width _ ha]
+  , h_height := by simp [r.h_height]}
+
+def Rect.tileVert (height : Nat) (r : Rect) (hr : r.height > 0) : Rect :=
+  { width := r.width, height
+  , lines := List.replicate (height / r.height + 1) r.lines |>.join.take height
+  , h_width   := by intro l hl
+                    have := List.mem_join.mp <| List.mem_take hl
+                    rcases this with ⟨l',hl',h⟩
+                    rw [List.mem_replicate] at hl'
+                    simp at hl'; cases hl'
+                    simp [r.h_width _ h]
+  , h_height  := by simp [-List.replicate, -List.join]
+                    apply Nat.min_eq_left
+                    simp [r.h_height]
+                    conv => lhs; rw [← Nat.div_add_mod (m := height) (n := r.height)]
+                    conv => rhs; rw [Nat.mul_comm _ r.height, Nat.mul_add, Nat.mul_one]
+                    apply Nat.add_le_add_left
+                    apply Nat.le_of_lt; apply Nat.mod_lt _ hr }
+
+def Rect.tileHorz (width : Nat) (r : Rect) (hr : r.width > 0) : Rect :=
+  { width, height := r.height
+  , lines := r.lines.map (List.replicate (width / r.width + 1) · |> String.join |>.take width)
+  , h_width   := by intro l hl
+                    have := List.mem_map.mp hl
+                    rcases this with ⟨l',hl',rfl⟩
+                    simp
+                    apply Nat.min_eq_right
+                    sorry
+  , h_height  := by simp [r.h_height] }
+
+def vbox (children : List Rect) (align : HAlign := .left)
+          (sep : Rect := space 1 0) (hsep : sep.width > 0 := by simp) : Rect :=
+  let width := children.foldr (max ·.width) 0
+  have : ∀ c, c ∈ children → c.width ≤ width := by
+    intro l hl
+    induction children
+    . simp at hl
+    . simp at hl ⊢
+      cases hl
+      . simp [*, Nat.le_max_left]
+      . apply Nat.le_trans _ (Nat.le_max_right ..)
+        simp [*] at *
+  match children with
+  | [] => space width 0
+  | c::cs => 
+    aux width cs (fun c hc => this c (List.Mem.tail _ hc))
+      (c.padWidth width (this c (List.Mem.head _)) align)
+      (by simp [Rect.padWidth])
+      (sep.tileHorz width hsep)
+      (by simp [Rect.tileHorz])
+where aux width children (h : ∀ c, c ∈ children → c.width ≤ width)
+          acc (hacc : acc.width = width)
+          sep (hsep : sep.width = width) :=
+  match children with
+  | [] => acc
+  | c::cs =>
+    have := h c (List.Mem.head _)
+    aux width cs (fun c hc => h c (List.Mem.tail _ hc))
+      (acc.joinVert sep (by simp [hacc, hsep])
+        |>.joinVert
+          (c.padWidth width this align)
+          (by simp [Rect.joinVert, Rect.padWidth, hacc]))
+      (by simp [Rect.joinVert, hacc])
+      sep hsep
+
+def hbox (children : List Rect) (align : VAlign := .top)
+          (sep : Rect := space 0 1) (hsep : sep.height > 0 := by simp) : Rect :=
+  let height := children.foldr (max ·.height) 0
+  have : ∀ c, c ∈ children → c.height ≤ height := by
+    intro l hl
+    induction children
+    . simp at hl
+    . simp at hl ⊢
+      cases hl
+      . simp [*, Nat.le_max_left]
+      . apply Nat.le_trans _ (Nat.le_max_right ..)
+        simp [*] at *
+  match children with
+  | [] => space 0 height
+  | c::cs =>
+    aux height cs (fun c hc => this c (List.Mem.tail _ hc))
+      (c.padHeight height (this c (List.Mem.head _)) align)
+      (by simp [Rect.padHeight])
+      (sep.tileVert height hsep)
+      (by simp [Rect.tileVert])
+where aux height children (h : ∀ c, c ∈ children → c.height ≤ height)
+          acc (hacc : acc.height = height) sep (hsep : sep.height = height) :=
+  match children with
+  | [] => acc
+  | c::cs =>
+    have := h c (List.Mem.head _)
+    aux height cs (fun c hc => h c (List.Mem.tail _ hc))
+      (acc.joinHorz sep (by simp [hacc, hsep])
+        |>.joinHorz
+          (c.padHeight height this align)
+          (by simp [Rect.joinHorz, Rect.padHeight, hacc]))
+      (by simp [Rect.joinHorz, hacc])
+      sep hsep
