C0deine/Utils/Symbol.lean
@@ -5,7 +5,7 @@ namespace C0deine
 structure Symbol where
   name : String
   id : UInt64
-deriving DecidableEq, Inhabited
+deriving DecidableEq, Inhabited, Repr
 
 instance : ToString Symbol where toString s := s.name
 instance : Hashable Symbol where hash s := s.id
